thys/MFODL_Monitor_Devel/Optimized_Agg_Temporal.thy
@@ -64,14 +64,16 @@ fun join_mmasaux :: "args \<Rightarrow> event_data table \<Rightarrow> mmasaux \
           tuple_since' = (if take_all then tuple_since else Mapping.empty) in
           ((t, gc, maskL, maskR, data_prev, data_in, table_in', wf_table_in', tuple_in', wf_table_since', tuple_since'), aggaux'))
        else (let wf_X = wf_table_of_idx (wf_idx_of_set (args_n args) (args_L args) (args_L args) X);
-          X_in = wf_table_set (wf_table_join wf_table_in wf_X);
-          (tuple_in', to_del_in) = filter_join' pos X_in tuple_in;
-          table_in' = table_in - to_del_in;
-          wf_table_in' = wf_table_antijoin wf_table_in (wf_table_of_set_args args to_del_in);
-          X_since = wf_table_set (wf_table_join wf_table_since wf_X);
-          (tuple_since', to_del_since) = filter_join' pos X_since tuple_since;
-          wf_table_since' = wf_table_antijoin wf_table_since (wf_table_of_set_args args to_del_since) in
-          ((t, gc, maskL, maskR, data_prev, data_in, table_in', wf_table_in', tuple_in', wf_table_since', tuple_since'), delete_maggaux' aggargs to_del_in aggaux)))))"
+          wf_in_del = (if pos then wf_table_antijoin else wf_table_join) wf_table_in wf_X;
+          in_del = wf_table_set wf_in_del;
+          tuple_in' = mapping_delete_set tuple_in in_del;
+          table_in' = table_in - in_del;
+          wf_table_in' = wf_table_antijoin wf_table_in wf_in_del;
+          wf_since_del = (if pos then wf_table_antijoin else wf_table_join) wf_table_since wf_X;
+          since_del = wf_table_set wf_since_del;
+          tuple_since' = mapping_delete_set tuple_since since_del;
+          wf_table_since' = wf_table_antijoin wf_table_since wf_since_del in
+          ((t, gc, maskL, maskR, data_prev, data_in, table_in', wf_table_in', tuple_in', wf_table_since', tuple_since'), delete_maggaux' aggargs in_del aggaux)))))"
 
 fun gc_join_mmasaux :: "args \<Rightarrow> event_data table \<Rightarrow> mmasaux \<Rightarrow> mmasaux" where
   "gc_join_mmasaux args X ((t, gc, maskL, maskR, data_prev, data_in, table_in, wf_table_in, tuple_in, wf_table_since, tuple_since), aux) =
@@ -242,14 +244,16 @@ proof -
     next
       case False
       let ?temp = "let wf_X = wf_table_of_idx (wf_idx_of_set (args_n args) (args_L args) (args_L args) rel1);
-          X_in = wf_table_set (wf_table_join wf_table_in wf_X);
-          (tuple_in', to_del_in) = filter_join' (args_pos args) X_in tuple_in;
-          table_in' = table_in - to_del_in;
-          wf_table_in' = wf_table_antijoin wf_table_in (wf_table_of_set_args args to_del_in);
-          X_since = wf_table_set (wf_table_join wf_table_since wf_X);
-          (tuple_since', to_del_since) = filter_join' (args_pos args) X_since tuple_since;
-          wf_table_since' = wf_table_antijoin wf_table_since (wf_table_of_set_args args to_del_since) in
-          ((nt, gc, maskL, maskR, data_prev, data_in, table_in', wf_table_in', tuple_in', wf_table_since', tuple_since'), delete_maggaux' aggargs to_del_in aggaux)"
+        wf_in_del = (if args_pos args then wf_table_antijoin else wf_table_join) wf_table_in wf_X;
+        in_del = wf_table_set wf_in_del;
+        tuple_in' = mapping_delete_set tuple_in in_del;
+        table_in' = table_in - in_del;
+        wf_table_in' = wf_table_antijoin wf_table_in wf_in_del;
+        wf_since_del = (if args_pos args then wf_table_antijoin else wf_table_join) wf_table_since wf_X;
+        since_del = wf_table_set wf_since_del;
+        tuple_since' = mapping_delete_set tuple_since since_del;
+        wf_table_since' = wf_table_antijoin wf_table_since wf_since_del in
+        ((nt, gc, maskL, maskR, data_prev, data_in, table_in', wf_table_in', tuple_in', wf_table_since', tuple_since'), delete_maggaux' aggargs in_del aggaux)"
       have *: "join_mmasaux args rel1 ((nt, gc, maskL, maskR, data_prev, data_in, table_in, wf_table_in, tuple_in, wf_table_since, tuple_since), aggaux) = ?temp" 
         using False some_aggargs by auto
       have "valid_mmasaux args cur ?temp (map (\<lambda>(t, rel). (t, join rel (args_pos args) rel1)) auxlist)" 
@@ -259,11 +263,19 @@ proof -
       next
         case (Some a)
         then have valid_maggaux: "valid_maggaux aggargs a (Mapping.keys tuple_in)" using some_aggargs assms(1) by auto
+        have L_R: "args_L args \<subseteq> args_R args"
+          and sig_in: "wf_table_sig wf_table_in = (args_n args, args_R args)"
+          and table_in: "wf_table_set wf_table_in = table_in"
+          using valid_msaux
+          by auto
+        note aux = trans[OF wf_table_sig_of_idx wf_idx_sig_of_set]
         show ?thesis using
             valid_delete_maggaux[OF valid_maggaux,
-              where ?Y="(table_in - Mapping.keys (filter_join (args_pos args) (wf_table_set (wf_table_join wf_table_in (wf_table_of_idx (wf_idx_of_set (args_n args) (args_L args) (args_L args) rel1)))) tuple_in))"]
+              where ?Y="wf_table_set ((if args_pos args then wf_table_antijoin else wf_table_join) wf_table_in (wf_table_of_idx (wf_idx_of_set (args_n args) (args_L args) (args_L args) rel1)))"]
               some_aggargs Some valid_msaux' False mapping_filter_keys_diff[of _ tuple_in, symmetric]
-          by (auto simp del:delete_maggaux.simps valid_mmsaux.simps simp: keys_in split:option.splits prod.splits if_splits)
+          by (auto simp del:delete_maggaux.simps valid_mmsaux.simps simp: keys_in table_in
+              wf_table_set_antijoin[OF sig_in aux L_R, unfolded join_sub[OF L_R wf_table_set_table[OF aux] wf_table_set_table[OF sig_in]]]
+              wf_table_set_join[OF sig_in aux refl, where ?A'="args_L args", unfolded join_sub[OF L_R wf_table_set_table[OF aux] wf_table_set_table[OF sig_in]]] split:option.splits prod.splits if_splits)
       qed
       then show ?thesis using * by presburger
     qed
